Start defining state array etc.

examples/Crypto/Keccak/keccakScript.sml
@@ -1,6 +1,108 @@
 open HolKernel Parse boolLib bossLib;
+open pairTheory listTheory rich_listTheory wordsTheory;
 
 val _ = new_theory "keccak";
 
-val _ = export_theory();
+Datatype:
+  state_array =
+  <| w: num
+   ; A: num # num # num -> bool
+   |>
+End
 
+val state_array_component_equality = theorem"state_array_component_equality";
+
+Definition wf_state_array_def:
+  wf_state_array a ⇔
+  ∀x y z. ¬(x < 5 ∧ y < 5 ∧ z < a.w) ⇒ ¬ a.A (x, y, z)
+End
+
+Definition Keccak_widths_def:
+  Keccak_widths = {25; 50; 100; 200; 400; 800; 1600}
+End
+
+fun pow2 n = if n = 0 then 1 else 2 * pow2 (n - 1)
+
+Theorem Keccak_widths_DIV_25:
+  w ∈ Keccak_widths ⇒ ∃n. w = 25 * n
+Proof
+  rw[Keccak_widths_def]
+  THENL (List.tabulate(7,
+    fn i => exists_tac(numSyntax.term_of_int(pow2 i)))
+  ) \\ simp[]
+QED
+
+Definition b2w_def:
+  b2w b = b DIV 25
+End
+
+Definition string_to_state_array_def:
+  string_to_state_array s =
+  let b = LENGTH s in
+  let w = b2w b in
+    <| w := w
+     ; A := λ(x, y, z). EL (w * (5 * y + x) + z) s
+     |>
+End
+
+Definition Lane_def:
+  Lane a (i, j) =
+    GENLIST (λw. a.A (i, j, w)) a.w
+End
+
+Theorem LENGTH_Lane[simp]:
+  LENGTH (Lane a x) = a.w
+Proof
+  Cases_on`x` \\ rw[Lane_def]
+QED
+
+Definition Plane_def:
+  Plane a j =
+    FLAT (GENLIST (λi. Lane a (i, j)) 5)
+End
+
+Theorem LENGTH_Plane[simp]:
+  LENGTH (Plane a j) = 5 * a.w
+Proof
+  rw[Plane_def]
+QED
+
+Definition state_array_to_string_def:
+  state_array_to_string a =
+    FLAT (GENLIST (Plane a) 5)
+End
+
+Theorem string_to_state_array_to_string:
+  LENGTH s = 25 * n ⇒
+  state_array_to_string (string_to_state_array s) = s
+Proof
+  rw[state_array_to_string_def, string_to_state_array_def,
+     Plane_def, Lane_def, b2w_def] \\
+  let
+    val thm = GENLIST_APPEND |> GSYM
+    val cnv = numSyntax.term_of_int
+    fun tac i =
+      thm |> Q.ISPECL_THEN[`λw. EL w s`, `n`, `^(cnv i) * n`]
+      mp_tac \\ simp[] \\ disch_then kall_tac
+    fun k n = if n = 25 then ALL_TAC else tac n \\ k (n + 1)
+  in
+    k 1
+  end \\
+  pop_assum (SUBST1_TAC o SYM) \\
+  simp[GENLIST_ID]
+QED
+
+(*
+Theorem state_array_to_string_to_state_array:
+  wf_state_array a ⇒
+  string_to_state_array (state_array_to_string a) = a
+Proof
+  rw[state_array_to_string_def, string_to_state_array_def, b2w_def,
+     state_array_component_equality, FUN_EQ_THM, FORALL_PROD,
+     wf_state_array_def]
+  \\ rw [Plane_def, Lane_def]
+  \\ rename1 `a.A (x, y, z)`
+  \\ Cases_on`x = 0` \\ fs[]
+*)
+
+val _ = export_theory();
